coq_translation/default/examples/generics/generics_bounds_test_case_empty_bounds.v
@@ -18,14 +18,14 @@ Definition Turkey := @Turkey.t.
 
 Module Red.
   Unset Primitive Projections.
-  Class Trait (Self : Set) : Type := {
+  Class Trait (Self : Set) `{State.Trait} : Type := {
   }.
   Global Set Primitive Projections.
 End Red.
 
 Module Blue.
   Unset Primitive Projections.
-  Class Trait (Self : Set) : Type := {
+  Class Trait (Self : Set) `{State.Trait} : Type := {
   }.
   Global Set Primitive Projections.
 End Blue.
